theories/clang/lib/list.v
@@ -18,6 +18,14 @@ Section proof.
                      p ↦ Vpair x l' @ tcell t ∗ isList l' xs' t)%I
     end.
 
+  Fixpoint isListSeg (l lt lt2: val) (x: val) (xs: list val) (t: type) :=
+    match xs with
+      | [] => (∃ p, ⌜ l = Vptr p ∧ l = lt ∧ typeof x t⌝ ∗ p ↦ Vpair x lt2 @ tcell t)%I
+      | x'::xs' => (∃ p l',
+                     ⌜ l = Vptr p ∧ typeof x t ∧ typeof l' (Tptr (tcell t)) ⌝ ∗
+                     p ↦ Vpair x l' @ tcell t ∗ isListSeg l' lt lt2 x' xs' t)%I
+    end.
+  
   Lemma isList_ptr (l: val) (xs: list val) (t: type) :
     isList l xs t ⊢ ⌜ typeof l (Tptr Tvoid) ⌝.
   Proof.
@@ -41,6 +49,7 @@ Section proof.
   Definition x: ident := 1.
   Definition y: ident := 2.
   Definition t: ident := 3.
+  Definition t': ident := 4.
 
   Notation "'Tlist'" := (Tptr (tcell Tint32)).
 
@@ -55,6 +64,166 @@ Section proof.
 
   Definition ps :=
     [ (x, Tlist); (y, Tptr Tvoid) ].
+
+  Definition traverse_list (lx: val) : expr :=
+    while [ !lx@Tlist != null ] (!lx@Tlist != null) <{ lx <- snd (!(!lx@Tlist)@(tcell Tint32)) }>.
+  
+  Lemma traverse_spec Φ lx xs: ∀ l,
+    lx ↦ l @ Tlist ∗ isList l xs Tint32 ∗ (isList l xs Tint32 -∗ Φ void)
+    ⊢ WP traverse_list lx {{ v, Φ v }}.
+  Proof.
+    induction xs as [|x xs' IHxs'].
+    - iIntros (l) "[? [% HΦ]]".
+      rewrite /traverse_list. subst.
+      wp_run. by iApply "HΦ".
+    - iIntros (l) "[Hlx [Hl HΦ]]".
+      simpl. iDestruct "Hl" as (p l') "[% [Hp Hl']]".
+      destruct_ands. subst.
+      rewrite /traverse_list. wp_load. wp_op. iApply wp_while_true. iNext.
+      wp_load. wp_load. wp_snd. iNext. wp_assign.
+      iApply IHxs'. iFrame. iIntros "?".
+      iApply "HΦ". iExists _, _. iFrame.
+      done.
+  Qed.
+
+  Lemma lseg_snoc' v:
+    typeof v Tint32 →
+    ∀ xs x p p' (p'': addr) l'',
+      typeof l'' Tlist →
+      isListSeg p p' p'' x xs Tint32 ∗ p'' ↦ Vpair v l'' @ tcell Tint32
+       ⊢ isListSeg p p'' l'' x (xs ++ [v]) Tint32.
+  Proof.
+    intros ?.
+    induction xs as [|x' xs' IHxs']; iIntros (x p p' p'' l'' ?) "[Hl Hv]"; simpl.
+    - iDestruct "Hl" as (p''') "[% ?]". destruct_ands. subst.
+      iExists p''', p''. iSplit=>//. iFrame.
+      iExists _. iFrame. done.
+    - iDestruct "Hl" as (p''' l') "[% [? ?]]". destruct_ands. subst.
+      specialize (IHxs' x' l' p' p'' l'').
+      iDestruct (IHxs' with "[~1 Hv]") as "?"=>//; first iFrame.
+      iExists _, _. iFrame. done.
+  Qed.
+
+  Lemma lseg_snoc v xs x p p' (p'': addr) l'':
+    typeof v Tint32 → typeof l'' Tlist →
+    isListSeg p p' p'' x xs Tint32 ∗ p'' ↦ Vpair v l'' @ tcell Tint32
+    ⊢ isListSeg p p'' l'' x (xs ++ [v]) Tint32.
+  Proof. iIntros (??) "?". iApply lseg_snoc'=>//. Qed.
+  
+  Lemma lseg_unsnoc: ∀ xs p (p': addr) x,
+    isListSeg p p' null x xs Tint32 ⊢
+    (∃ (x': val) xs' p'', isListSeg p p'' p' x xs' Tint32 ∗
+     p' ↦ Vpair x' null @ tcell Tint32 ∗ ⌜ xs = xs' ++ [x'] ⌝ ) ∨
+    (⌜ p = p' ∧ xs = [] ⌝ ∗ p' ↦ Vpair x null @ tcell Tint32).
+  Proof.
+    induction xs as [|x' xs' IHxs'].
+    - iIntros (???) "H". simpl. iDestruct "H" as (?) "[% ?]". destruct_ands. simplify_eq.
+      iRight. by iFrame.
+    - iIntros (???) "H". simpl. iDestruct "H" as (??) "[% [? ?]]". destruct_ands. simplify_eq.
+      iDestruct (IHxs' with "~1") as "[?|[% ?]]".
+      + iLeft. iDestruct "~2" as (???) "[? [? %]]". iExists H2. iFrame.
+        subst. iExists (x'::H5). iExists _.
+        iSplit=>//. simpl. iExists _, _.
+        iFrame. done.
+      + destruct_ands. subst. iLeft. iExists x'. iFrame.
+        iExists [], H0. iSplit=>//. simpl. iExists _.
+        iSplit=>//.
+  Qed.
+
+  Lemma lseg_to_list xs: ∀ p p' x,
+    isListSeg p p' null x xs Tint32 ⊢ isList p (x::xs) Tint32.
+  Proof.
+    induction xs as [|x' xs' IHxs'].
+    - iDestruct 1 as (?) "[% ?]". destruct_ands. subst.
+      iExists _, _. iFrame. iSplit=>//.
+    - simpl. iDestruct 1 as (??) "[% [? ?]]". destruct_ands. subst.
+      iDestruct (IHxs' with "~") as "?".
+      iExists _, _. iFrame. iSplit=>//.
+  Qed.
+  
+  Lemma enq_spec' lx (p: addr) Φ x xs: ∀ xs2 xs1 pt pt' (p': addr) l',
+    typeof l' Tlist → typeof p Tlist →
+    lx ↦ p @ Tlist ∗ pt ↦ p' @ Tlist ∗ pt' ↦ l' @ Tlist ∗
+    isListSeg p p' l' x xs1 Tint32 ∗ isList l' xs2 Tint32 ∗ ⌜ xs = xs1 ++ xs2 ⌝ ∗
+    (∀ p': addr, lx ↦ p @ Tlist -∗ pt ↦ p' @ Tlist -∗ isListSeg p p' null x xs Tint32 -∗
+                 pt' ↦ null @ Tlist -∗ Φ void)
+    ⊢ WP (while [! pt' @ Tlist != null](! pt' @ Tlist != null)<{
+            pt <- ! pt' @ Tlist ;; pt' <- snd ! ! pt' @ Tlist @ (tcell Tint32)
+          }>) {{ Φ }}.
+  Proof.
+    induction xs2 as [|x' xs2' IHxs']; iIntros (???????) "(Hlx&Hpt&Hpt'&Hxs1&Hxs2&%&HΦ)".
+    - iDestruct "Hxs2" as "%". subst.
+      wp_run. rewrite (right_id_L _ (++)).
+      by iSpecialize ("HΦ" $! p' with "Hlx Hpt Hxs1 Hpt'").
+    - simpl. wp_load. iDestruct "Hxs2" as (p'' l'') "[% [? ?]]".
+      destruct_ands. subst. wp_op. iApply wp_while_true.
+      iNext. wp_load. wp_assign. wp_load. wp_load.
+      wp_snd. iNext. wp_assign.
+      iApply (IHxs' (xs1 ++ [x'])); last iFrame; auto.
+      iSplitL.
+      { iApply lseg_snoc=>//. iFrame. }
+      { by rewrite -assoc. }
+  Qed.
+  
+  Definition enq_list (lx: val) (v: val) : expr :=
+    let: t ::: Tlist := Ealloc Tlist (!lx@Tlist) in
+    Eif (t != null) (
+      let: t' ::: Tlist := Ealloc Tlist (snd (!?t)) in
+      while [ t' != null ] (t' != null) <{
+        t <- t';;
+        t' <- snd (!?t')
+      }> ;;
+      snd !?t <- Ealloc (tcell Tint32) (Vpair v null)
+    ) (* else *) (
+      lx <- Ealloc (tcell Tint32) (Vpair v null)
+    ).
+
+  Lemma enq_spec Φ lx xs v: typeof v Tint32 → ∀ l,
+    lx ↦ l @ Tlist ∗ isList l xs Tint32 ∗
+    (∀ l', (lx ↦ l' @ Tlist) -∗ (isList l' (xs ++ [v]) Tint32) -∗ Φ void)
+    ⊢ WP enq_list lx v {{ v, Φ v }}.
+  Proof.
+    intros ?. rewrite /enq_list. subst.
+    unfold Edecl. iIntros (l) "[Hlx [Hl HΦ]]". wp_load.
+    iDestruct (mapsto_typeof with "Hlx") as "%".
+    wp_alloc pt as "Ht". wp_let. destruct xs as [|x xs'] eqn:?; subst.
+    - simpl. iDestruct "Hl" as "%". subst. wp_run. iApply wp_if_false.
+      wp_run. wp_alloc p as "Hp"=>//.
+      wp_assign. iApply ("HΦ" with "[-Hp]")=>//.
+      iExists _, _. iFrame. iSplit=>//.
+    - simpl. wp_load. iDestruct "Hl" as (p l') "[% [? ?]]".
+      destruct_ands. subst.
+      wp_op. iApply wp_if_true.
+      iNext. wp_load. wp_load. wp_snd. iNext.
+      wp_alloc pt' as "Hpt'". wp_let.
+      iApply wp_seq=>//.
+      iApply (enq_spec' lx p _ x _ _ [] pt pt' p l'); last iFrame; auto.
+      iSplitL "~".
+      { simpl. iExists _. iSplit=>//. }
+      iSplit=>//. iIntros (?) "? ? ? ?".
+      wp_skip. destruct a. wp_load. wp_op.
+      rewrite /offset_by_byte.
+      replace (Z.to_nat (Byte.intval (Byte.repr 4))) with 4%nat; last done.
+      iDestruct (lseg_unsnoc with "~2") as "[H|[% Hp]]".
+      + iDestruct "H" as (???) "[Hl [Hp %]]". destruct_ands. subst.
+        iDestruct (mapstoval_split with "Hp") as "[Hp1 Hp2]". simpl.
+        wp_alloc lp' as "Hlp'"=>//. wp_assign.
+        iApply ("HΦ" with "~").
+        iDestruct (mapsto_typeof with "Hp1") as "%".
+        iDestruct (mapstoval_join with "[Hp1 Hp2]") as "Hp"; first by iSplitL "Hp1".
+        iDestruct (lseg_snoc with "[Hl Hp]") as "Hl'"; try iFrame; auto.
+        iDestruct (lseg_snoc with "[Hl' Hlp']") as "Hl''"; try iFrame; auto.
+        iDestruct (lseg_to_list with "Hl''") as "Hl''".
+        simpl. iDestruct "Hl''" as (??) "[% [? ?]]". destruct_ands. simplify_eq.
+        iExists _, _. iFrame. done.
+      + destruct_ands. subst.
+        iDestruct (mapstoval_split with "Hp") as "[Hp1 Hp2]". simpl.
+        wp_alloc lp' as "Hlp'"=>//. wp_assign.
+        iApply ("HΦ" with "~").
+        iDestruct (mapstoval_join with "[Hp1 Hp2]") as "Hp"; first by iSplitL "Hp1".
+        iExists _, _. iFrame. iSplit=>//.
+        iExists _, _. iFrame. iSplit=>//.
+  Qed.
 
   Lemma rev_spec' (f: ident) ks Φ px py pt xs:
     ∀ lx ly ys,
@@ -97,8 +266,6 @@ Section proof.
       by rewrite -app_assoc.
   Qed.
 
-
-  
   Lemma rev_spec (f: ident) ks Φ xs:
     ∀ lx ly ys,
       text_interp f (Function Tvoid ps rev_list) ∗
